

## Assignment-2

$$P(y|n) = b(y) \exp[nT(y) - a(n)]$$

~~$$P(y|k) = \frac{y^k e^{-k}}{k!}$$~~

$$P(y|\lambda) = \frac{\lambda^y e^{-\lambda}}{y!}$$

$$\frac{1}{y!} \exp(y \log \lambda - \lambda)$$

$$b(y) = \frac{1}{y!} \quad \begin{matrix} \text{(only one y)} \\ n^T = n = \log \lambda \end{matrix} \quad T(y) = y$$
$$a(n) = \lambda = e^n$$

2) Let  $\phi_k$  is prob. of output  $y_k$

We define  $T(y) \in \mathbb{R}^{k-1}$

$$T(1) = \begin{bmatrix} 1 \\ 0 \\ \vdots \\ 0 \end{bmatrix} \quad T(2) = \begin{bmatrix} 0 \\ 1 \\ \vdots \\ 0 \end{bmatrix} \quad \dots \quad T(k) = \begin{bmatrix} 0 \\ 0 \\ \vdots \\ 1 \end{bmatrix}$$

$$\phi_i = E[(T(y))_i] = P(y=i) \quad \text{where}$$

$$(T(y))_i = \begin{cases} 1 & \text{if } y=i \\ 0 & \text{otw} \end{cases}$$



$$P(y|\phi) = \phi_1^{(T(y))_1} \phi_2^{(T(y))_2} \dots \phi_k^{1 - \sum_{i=1}^{k-1} (T(y))_i}$$

$$= \exp \left( (T(y))_1 \log \left( \frac{\phi_1}{\phi_k} \right) \dots \right)$$

$$= b(y) \exp(n_T T(y) - a(\eta))$$

$$\eta = \begin{bmatrix} \log \left( \frac{\phi_1}{\phi_k} \right) \\ \vdots \\ \log \left( \frac{\phi_{k-1}}{\phi_k} \right) \end{bmatrix}$$

$$a(\eta) = -\log(\phi_k)$$

$$b(y) = 1$$

$$\eta_i = \log \frac{\phi_i}{\phi_k}$$

$$e^{\eta_i} = \frac{\phi_i}{\phi_k} \quad \phi_i = \phi_k e^{\eta_i}$$

$$\sum \phi_k e^{\eta_i} = \sum \phi_i = 1$$

$$\phi_k = \frac{1}{\sum e^{\eta_i}}$$

$$\phi_i = \frac{e^{\eta_i}}{\sum_{j=1}^k e^{\eta_j}}$$